src/program_proof/pav/invs.v
@@ -1,0 +1,82 @@
+From Perennial.program_proof Require Import grove_prelude.
+
+From Perennial.program_proof.pav Require Import common cryptoffi merkle rpc.
+From iris.unstable.base_logic Require Import mono_list.
+From Perennial.base_logic.lib Require Import ghost_map.
+From Perennial.algebra Require Import ghost_map_pers.
+
+Section epochChain.
+Context `{!heapGS Σ}.
+
+Definition chainSepNone_hashes_to h : iProp Σ :=
+  is_hash [(W8 0)] h.
+
+Definition binds (data links : list (list w8)) : iProp Σ :=
+  ∃ init,
+  "%Hinit" ∷ ⌜ links !! 0 = Some init ⌝ ∗
+  "#Hinit_hash" ∷ chainSepNone_hashes_to init ∗
+  (* every link except init was formed by the previous link. *)
+  "#Hbinds" ∷ ([∗ list] epoch ↦ d; l ∈ data; (drop 1 links),
+    ∃ prevLink,
+    ⌜ links !! epoch = Some prevLink ⌝ ∗
+    is_hash (chainSepSome.encodesF (chainSepSome.mk epoch prevLink d)) l).
+
+(* Can't state this thru stdpp Inj bc data, links related thru iProp, not pure func.
+Maybe if we had a pure hash func, things would be diff. *)
+Lemma binds_inj data0 data1 links0 links1 :
+  binds data0 links0 -∗
+  binds data1 links1 -∗
+  ⌜ data0 = data1 ↔ links0 = links1 ⌝.
+Proof. Admitted.
+End epochChain.
+
+Section global_inv.
+Context `{!heapGS Σ, !mono_listG gname Σ, !ghost_mapG Σ (list w8) (list w8)}.
+(* state is tied together as follows, all from one γ:
+γ →[mono_list]
+γtrees →[ghost_map_auth]
+trees →[is_tree_dig]
+digs →[binds]
+links. *)
+Definition global_inv γ : iProp Σ :=
+  ∃ γtrees trees updates digs links,
+  "HmonoTrees" ∷ mono_list_auth_own γ (1/2) γtrees ∗
+  "Htree_views" ∷ ([∗ list] γtr; tr ∈ γtrees; (trees ++ [updates]),
+    ghost_map_auth γtr (1/2) tr) ∗
+  "#Hdigs" ∷ ([∗ list] tr; dig ∈ trees; digs, is_tree_dig tr dig) ∗
+  "#Hdigs_links" ∷ binds digs links.
+End global_inv.
+
+Section serv_sigpreds.
+Context `{!heapGS Σ, !mono_listG gname Σ, !ghost_mapG Σ (list w8) (list w8)}.
+
+Definition serv_sigpred_link γ (data : servSepLink.t) : iProp Σ :=
+  ∃ (epoch : w64) (prevLink dig : list w8) γtrees trees digs links,
+  "#Hbind" ∷ is_hash (chainSepSome.encodesF (chainSepSome.mk epoch prevLink dig)) data.(servSepLink.link) ∗
+  "#HmonoIdx" ∷ mono_list_lb_own γ γtrees ∗
+  "#Htree_views" ∷ ([∗ list] γtr; tr ∈ γtrees; trees,
+    ghost_map_auth_pers γtr tr) ∗
+  "#Hdigs" ∷ ([∗ list] tr; dig ∈ trees; digs, is_tree_dig tr dig) ∗
+  "#Hdigs_links" ∷ binds digs links ∗
+  "%Hlink_look" ∷ ⌜ links !! (uint.nat epoch) = Some data.(servSepLink.link) ⌝.
+
+Definition serv_sigpred_put γ (data : servSepPut.t) : iProp Σ :=
+  ∃ γtr,
+  "#Htr_idx" ∷ mono_list_idx_own γ (uint.nat data.(servSepPut.epoch)) γtr ∗
+  "#Hentry" ∷ data.(servSepPut.id) ↪[γtr]□ data.(servSepPut.val).
+
+Definition serv_sigpred γ : (list w8 → iProp Σ) :=
+  λ data,
+    (inv nroot (global_inv γ) ∗
+    ((
+      ∃ dataSepLink,
+      ⌜servSepLink.encodes data dataSepLink⌝ ∗
+      serv_sigpred_link γ dataSepLink
+    )%I
+    ∨
+    (
+      ∃ dataSepPut,
+      ⌜servSepPut.encodes data dataSepPut⌝ ∗
+      serv_sigpred_put γ dataSepPut
+    )%I))%I.
+End serv_sigpreds.
